better notation for exists vprops

pulse/examples/dsls/mini_steel/tests/Pulse.Tests.fst
@@ -15,153 +15,154 @@ module U32 = FStar.UInt32
 let expects = ()
 let provides = ()
 let while = ()
+let intro = ()
+// [@@ expect_failure]
+// %splice_t[tuple_test] (check (`(
+//   fun (r:ref (U32.t & U32.t)) (n1:erased U32.t) (n2:erased U32.t) ->
+//            (expects (pts_to r full_perm (reveal n1, reveal n2)))
+//     (provides (fun _ -> pts_to r full_perm (reveal n1, reveal n2)))
+//     (
+//       read #(U32.t & U32.t) r
+//     )
+// )))
 
-[@@ expect_failure]
-%splice_t[tuple_test] (check (`(
-  fun (r:ref (U32.t & U32.t)) (n1:erased U32.t) (n2:erased U32.t) ->
-           (expects (pts_to r full_perm (reveal n1, reveal n2)))
-    (provides (fun _ -> pts_to r full_perm (reveal n1, reveal n2)))
-    (
-      read #(U32.t & U32.t) r
-    )
-)))
+// (* Start up the solver and feed it the initial context *)
+// let warmup (x:int) = assert (x + 1 > x)
 
-(* Start up the solver and feed it the initial context *)
-let warmup (x:int) = assert (x + 1 > x)
+// %splice_t[test_true] (check (`(true)))
 
-%splice_t[test_true] (check (`(true)))
-
-%splice_t[test_write_10] (check  (`(
-   fun (x:ref UInt32.t)
-     (#n:erased UInt32.t) -> 
-     (expects (
-        pts_to x full_perm n))
-     (provides (fun _ ->
-        pts_to x full_perm 0ul))
-     (
-       write x 1ul;
-       write x 0ul
-     )
-   )))
-
-
-%splice_t[test_read] (check (`(
-  fun (r:ref UInt32.t)
-    (#n:erased UInt32.t) (#p:perm) ->
-    (expects (
-       pts_to r p n))
-    (provides (fun x ->
-       pts_to r p x))
-    (
-       read #U32.t r
-    )
-)))
-
-//Bound variable escapes scope
-[@@ expect_failure]
-%splice_t[test_read_alt_write] (check (`(
-  fun (r:ref UInt32.t)
-    (#n:erased UInt32.t) ->
-    (expects (
-       pts_to r full_perm n))
-    (
-       let x = read #U32.t r in
-       write r x
-    )
-)))
+// %splice_t[test_write_10] (check  (`(
+//    fun (x:ref UInt32.t)
+//      (#n:erased UInt32.t) -> 
+//      (expects (
+//         pts_to x full_perm n))
+//      (provides (fun _ ->
+//         pts_to x full_perm 0ul))
+//      (
+//        write x 1ul;
+//        write x 0ul
+//      )
+//    )))
 
 
-%splice_t[swap] (check (`(
-  fun (r1 r2:ref UInt32.t)
-    (#n1 #n2:erased UInt32.t) ->
-    (expects  (
-      pts_to r1 full_perm n1 `star` 
-      pts_to r2 full_perm n2))
-    (provides (fun _ ->
-      pts_to r1 full_perm n2 `star` 
-      pts_to r2 full_perm n1))
-    (
-      let x = read #U32.t r1 in
-      let y = read #U32.t r2 in
-      write r1 y;
-      write r2 x
-    )
-)))
+// %splice_t[test_read] (check (`(
+//   fun (r:ref UInt32.t)
+//     (#n:erased UInt32.t) (#p:perm) ->
+//     (expects (
+//        pts_to r p n))
+//     (provides (fun x ->
+//        pts_to r p x))
+//     (
+//        read #U32.t r
+//     )
+// )))
+
+// //Bound variable escapes scope
+// [@@ expect_failure]
+// %splice_t[test_read_alt_write] (check (`(
+//   fun (r:ref UInt32.t)
+//     (#n:erased UInt32.t) ->
+//     (expects (
+//        pts_to r full_perm n))
+//     (
+//        let x = read #U32.t r in
+//        write r x
+//     )
+// )))
 
 
-%splice_t[call_swap2] (check (`(
-  fun (r1 r2:ref UInt32.t)
-    (#n1 #n2:erased UInt32.t) ->
-    (expects  (
-      pts_to r1 full_perm n1 `star` 
-      pts_to r2 full_perm n2))
-    (provides (fun _ -> 
-      pts_to r1 full_perm n1 `star` 
-      pts_to r2 full_perm n2))
-    (
-      swap r1 r2;
-      swap r1 r2
-    )
-)))
+// %splice_t[swap] (check (`(
+//   fun (r1 r2:ref UInt32.t)
+//     (#n1 #n2:erased UInt32.t) ->
+//     (expects  (
+//       pts_to r1 full_perm n1 `star` 
+//       pts_to r2 full_perm n2))
+//     (provides (fun _ ->
+//       pts_to r1 full_perm n2 `star` 
+//       pts_to r2 full_perm n1))
+//     (
+//       let x = read #U32.t r1 in
+//       let y = read #U32.t r2 in
+//       write r1 y;
+//       write r2 x
+//     )
+// )))
 
 
-//
-// swap with elim_pure, bind of ghost and stt
-//
+// %splice_t[call_swap2] (check (`(
+//   fun (r1 r2:ref UInt32.t)
+//     (#n1 #n2:erased UInt32.t) ->
+//     (expects  (
+//       pts_to r1 full_perm n1 `star` 
+//       pts_to r2 full_perm n2))
+//     (provides (fun _ -> 
+//       pts_to r1 full_perm n1 `star` 
+//       pts_to r2 full_perm n2))
+//     (
+//       swap r1 r2;
+//       swap r1 r2
+//     )
+// )))
 
-%splice_t[swap_with_elim_pure] (check (`(
-  fun (r1:ref UInt32.t) (r2:ref UInt32.t) (n1:erased UInt32.t) (n2:erased UInt32.t) ->
-    (expects (pts_to r1 full_perm n1 `star` pts_to r2 full_perm n2))
-    (provides (fun _ ->
-               pts_to r1 full_perm n2 `star` pts_to r2 full_perm n1))
-    (
-      let x = read_pure #U32.t r1 in
-      let y = read_pure #U32.t r2 in
-      write r1 y;
-      write r2 x
-    )
-)))
 
-%splice_t[swap_with_elim_pure_and_atomic] (check (`(
-  fun (r1:ref UInt32.t) (r2:ref UInt32.t) (n1:erased UInt32.t) (n2:erased UInt32.t) ->
-    (expects (pts_to r1 full_perm n1 `star` pts_to r2 full_perm n2))
-    (provides (fun _ ->
-               pts_to r1 full_perm n2 `star` pts_to r2 full_perm n1))
-    (
-      let x = read_atomic r1 in
-      let y = read_atomic r2 in
-      write_atomic r1 y;
-      write_atomic r2 x
-    )
-)))
+// //
+// // swap with elim_pure, bind of ghost and stt
+// //
 
-%splice_t[intro_pure_example] (check (`(
-  fun (r:ref UInt32.t) (n1:erased UInt32.t) (n2:erased UInt32.t) ->
-    (expects (pts_to r full_perm n1 `star` pure (eq2_prop (reveal n1) (reveal n2))))
-    (provides (fun x -> pts_to r full_perm n2 `star` pure (eq2_prop (reveal n2) (reveal n1))))
-    (
-       ()
-    )
-)))
+// %splice_t[swap_with_elim_pure] (check (`(
+//   fun (r1:ref UInt32.t) (r2:ref UInt32.t) (n1:erased UInt32.t) (n2:erased UInt32.t) ->
+//     (expects (pts_to r1 full_perm n1 `star` pts_to r2 full_perm n2))
+//     (provides (fun _ ->
+//                pts_to r1 full_perm n2 `star` pts_to r2 full_perm n1))
+//     (
+//       let x = read_pure #U32.t r1 in
+//       let y = read_pure #U32.t r2 in
+//       write r1 y;
+//       write r2 x
+//     )
+// )))
 
-%splice_t[if_example] (check (`(
-  fun (r:ref UInt32.t) (n:erased UInt32.t{eq2_prop (U32.v (reveal n)) 1}) (b:bool) ->
-    (expects (pts_to r full_perm n))
-    (provides (fun _ -> pts_to r full_perm (U32.add (reveal n) 2ul)))
-    (
-      let x = read_atomic r in
-      if b
-      then write r (U32.add x 2ul)
-      else write_atomic r 3ul
-    )
-)))
+// %splice_t[swap_with_elim_pure_and_atomic] (check (`(
+//   fun (r1:ref UInt32.t) (r2:ref UInt32.t) (n1:erased UInt32.t) (n2:erased UInt32.t) ->
+//     (expects (pts_to r1 full_perm n1 `star` pts_to r2 full_perm n2))
+//     (provides (fun _ ->
+//                pts_to r1 full_perm n2 `star` pts_to r2 full_perm n1))
+//     (
+//       let x = read_atomic r1 in
+//       let y = read_atomic r2 in
+//       write_atomic r1 y;
+//       write_atomic r2 x
+//     )
+// )))
 
+// %splice_t[intro_pure_example] (check (`(
+//   fun (r:ref UInt32.t) (n1:erased UInt32.t) (n2:erased UInt32.t) ->
+//     (expects (pts_to r full_perm n1 `star` pure (eq2_prop (reveal n1) (reveal n2))))
+//     (provides (fun x -> pts_to r full_perm n2 `star` pure (eq2_prop (reveal n2) (reveal n1))))
+//     (
+//        ()
+//     )
+// )))
+
+// %splice_t[if_example] (check (`(
+//   fun (r:ref UInt32.t) (n:erased UInt32.t{eq2_prop (U32.v (reveal n)) 1}) (b:bool) ->
+//     (expects (pts_to r full_perm n))
+//     (provides (fun _ -> pts_to r full_perm (U32.add (reveal n) 2ul)))
+//     (
+//       let x = read_atomic r in
+//       if b
+//       then write r (U32.add x 2ul)
+//       else write_atomic r 3ul
+//     )
+// )))
+
+//#push-options "--ugly --print_implicits"
 %splice_t[elim_intro_exists] (check (`(
   fun (r:ref UInt32.t) ->
-    (expects (exists_ (fun n -> pts_to r full_perm n)))
-    (provides (fun _ -> exists_ (fun n -> pts_to r full_perm n)))
+    (expects (exists n. pts_to r full_perm n))
+    (provides (fun _ -> exists n. pts_to r full_perm n))
     (
-      intro_exists (fun n -> pts_to r full_perm n) _
+      intro (exists n. pts_to r full_perm n) _
     )
 )))
 
@@ -182,20 +183,20 @@ let warmup (x:int) = assert (x + 1 > x)
 
 %splice_t[while_test] (check (`(
   fun (r:ref UInt32.t) ->
-    (expects (exists_ (fun (b:bool) -> exists_ (fun (n:UInt32.t) -> pts_to r full_perm n))))
-    (provides (fun _ -> exists_ (fun (n:UInt32.t) -> pts_to r full_perm n)))
+    (expects (exists (b:bool) n. pts_to r full_perm n))
+    (provides (fun _ -> exists n. pts_to r full_perm n))
     (
-      intro_exists (fun n -> pts_to r full_perm n) _;
-      intro_exists (fun (b:bool) -> exists_ (fun n -> pts_to r full_perm n)) false;    
+      intro (exists n. pts_to r full_perm n) _;
+      intro (exists (b:bool) n. pts_to r full_perm n) false;
       while
-        (fun b -> exists_ (fun (n:UInt32.t) -> pts_to r full_perm n))
+        (fun b -> exists n. pts_to r full_perm n)
         (
-          intro_exists (fun n -> pts_to r full_perm n) _;
+          intro (exists n. pts_to r full_perm n) _;
           return_stt_noeq true
         )
         (
-          intro_exists (fun n -> pts_to r full_perm n) _;        
-          intro_exists (fun (b:bool) -> exists_ (fun n -> pts_to r full_perm n)) true;
+          intro (exists n. pts_to r full_perm n) _;
+          intro (exists (b:bool) n. pts_to r full_perm n) true;          
           return_stt_noeq ()
         )
     )
@@ -205,16 +206,16 @@ let warmup (x:int) = assert (x + 1 > x)
 
 %splice_t[while_count] (check (`(
   fun (r:ref UInt32.t) ->
-    (expects (exists_ (fun n -> pts_to r full_perm n)))
+    (expects (exists n. pts_to r full_perm n))
     (provides (fun _ -> pts_to r full_perm 10ul))
     (
     //      let n = elim_exists _ in
-      let x = read_pure r in
+      let x = read_pure #U32.t r in
       // let b = return_stt (x <> 10ul) in
       let _ =
         // let reveal_n = stt_ghost_reveal UInt32.t n in
-        intro_exists (fun n -> pts_to r full_perm n `star` pure (eq2_prop (n <> 10ul) (n <> 10ul))) _; //reveal_n;
-        intro_exists (fun b -> exists_ (fun n -> pts_to r full_perm n `star` pure (eq2_prop b (n <> 10ul)))) _ in
+        intro (exists n. pts_to r full_perm n `star` pure (eq2_prop (n <> 10ul) (n <> 10ul))) _; //reveal_n;
+        intro (exists b n. pts_to r full_perm n `star` pure (eq2_prop b (n <> 10ul))) _ in
 
       stt_admit unit))))
 //       while
